a refinement with fresh vars for defun

shiftreset/Logic.v
@@ -1721,6 +1721,12 @@ Definition can_weaken_env f := forall s1 s2 h1 h2 R x u,
   satisfies s1 s2 h1 h2 R f ->
   satisfies (Fmap.update s1 x u) (Fmap.update s2 x u) h1 h2 R f.
 
+Definition can_weaken_env_fresh f := forall s1 s2 h1 h2 R x u,
+  ~ Fmap.indom s1 x ->
+  ~ Fmap.indom s2 x ->
+  satisfies s1 s2 h1 h2 R f ->
+  satisfies (Fmap.update s1 x u) (Fmap.update s2 x u) h1 h2 R f.
+
 Lemma weaken_req : forall H f,
   can_weaken_env f ->
   can_weaken_env (req H f).
@@ -1741,12 +1747,19 @@ Proof.
 Qed.
 
 Lemma weaken_defun : forall x u,
-  can_weaken_env (defun x u).
+  can_weaken_env_fresh (defun x u).
 Proof.
-  unfold can_weaken_env. intros.
-  inverts H as H. destr H.
-  (* apply s_ens. *)
-  (* exs. splits*. *)
+  unfold can_weaken_env_fresh. intros.
+  inverts H1 as H1.
+  unfold Fmap.update in H0.
+  lets: Fmap.disjoint_single_of_not_indom u0 H0.
+  apply s_defun.
+  { apply* not_indom_update.
+    rewrite Fmap.disjoint_union_eq_r in H2. destr H2.
+    apply disjoint_single_neq in H3.
+    congruence. }
+  { unfold Fmap.update.
+    fmap_eq. }
 Qed.
 
 Lemma weaken_seq : forall f1 f2,
@@ -1765,7 +1778,8 @@ Lemma weaken_rs : forall f r,
   can_weaken_env (rs f r).
 Proof.
   unfold can_weaken_env. intros.
-  inverts H0 as H0.
+  Abort.
+  (* inverts H0 as H0.
   { eapply s_rs_sh.
     eauto.
 
@@ -1776,7 +1790,7 @@ Proof.
   { apply s_rs_val.
     eauto. }
 (* Qed. *)
-Abort.
+Abort. *)
 
 Lemma weaken_ex : forall c,
   (forall x1, can_weaken_env (c x1)) ->
@@ -1795,8 +1809,7 @@ Proof.
   unfold can_weaken_env. intros.
   apply s_fall. intros b.
   inverts H0 as H0. specializes H0 b.
-  apply H.
-  eauto.
+  applys* H.
 Qed.
 
 Definition can_strengthen_env f := forall s1 s2 h1 h2 R x u,
